update recursion dataset

autogenerate.cpp
@@ -3,17 +3,40 @@
 using namespace std;
 
 int main() {
-    for (int i = 1; i <= 30; i++) {
+    /*for (int i = 31; i <= 40; i++) {
         cout << "Definition hash_" << i << "_correct_def (ll: LedgerLRecord rec) : Prop." << endl;
         cout << "execs0 (hash_" << i << " rec def) :" << endl;
         cout << "ll | \"m_string\" \"m_modulo\" \"m_multiplier\" -> l1 | \"m_hash\"." << endl;
         cout << "con (m_hash = fst (reference_hash_implementation " << i << "%nat m_string (uint2N m_multiplier) (uint2N m_modulo)))." << endl;
         cout << "Defined." << endl;
         cout << endl;
-    }
+    }*/
 
-    /*for (int i = 11; i <= 30; i++) {
-        cout << "#[returns=ret_]" << endl;
+    /*string s;
+    cin >> s;*/
+    for (int i = 40; i >= 3; i--) {
+        cout << "find . -type f -name \"*.v\" -print0 | xargs -0 sed -i \"s/";
+        for (int j = 1; j < i; j++) {
+            cout << "@hash_" << j;
+        }
+        cout << "/";
+        for (int j = i - 1; j >= 1; j--) {
+            cout << "@hash_" << j << " ";
+        }
+        cout << "/g\"" << endl;
+
+        /*cout << "Lemma hash_" << i << "_prf (ll : LedgerLRecord rec) : hash_" << i << "_correct_def ll." << endl;
+        cout << "start_proof; hash_" << i << "_start; prepare ll P loc_." << endl;
+        cout << "continue_all ";
+        for (int j = 1; j < i; j++) {
+            cout << "@hash_" << j;
+        }
+        cout << "." << endl;
+        cout << "time \"[simple][" << s << "][" << i << "]\" timeout 300 solver." << endl;
+        cout << "Time Qed." << endl;
+        cout << endl;*/
+
+        /*cout << "#[returns=ret_]" << endl;
         cout << "Ursus Definition hash_" << i << ": UExpression (uint64 * uint64) false." << endl;
         cout << "{" << endl;
         cout << "    ::// [m_current_power, m_hash] := hash_" << i - 1 << "()." << endl;
@@ -24,9 +47,9 @@ int main() {
         cout << "return." << endl;
         cout << "Defined." << endl;
         cout << "Sync." << endl;
-        cout << endl;
+        cout << endl;*/
 
-        cout << "Ursus Definition hash_" << i << ": UExpression PhantomType false." << endl;
+        /*cout << "Ursus Definition hash_" << i << ": UExpression PhantomType false." << endl;
         cout << "{" << endl;
         cout << "    ::// var00 current_power: uint64 := {1} ;_|." << endl; 
         cout << "    ::// m_hash := {0} ;_|." << endl;
@@ -45,6 +68,6 @@ int main() {
         cout << "return." << endl;
         cout << "Defined." << endl;
         cout << "Sync." << endl;
-        cout << endl;
-    }*/
+        cout << endl;*/
+    }
 }
