src/Recursion/Recursion.v
@@ -34,6 +34,7 @@ Local Open Scope N_scope.
 #[returns=ret_]
 Ursus Definition hash_1: UExpression (uint64 * uint64) false.
 {
+    ::// m_hash := {0}.
     ::// m_current_power := {1}.
     ::// m_hash := (m_hash + m_string[[{0}]] * m_current_power) % m_modulo.
     ::// ret_ := [m_current_power, m_hash] |.
@@ -144,6 +145,366 @@ Ursus Definition hash_10: UExpression (uint64 * uint64) false.
     ::// [m_current_power, m_hash] := hash_9().
     ::// m_current_power := (m_current_power * m_multiplier) % m_modulo.
     ::// m_hash := (m_hash + m_string[[{9}]] * m_current_power) % m_modulo.
+    ::// ret_ := [m_current_power, m_hash] |.
+}
+return.
+Defined.
+Sync.
+
+#[returns=ret_]
+Ursus Definition hash_11: UExpression (uint64 * uint64) false.
+{
+    ::// [m_current_power, m_hash] := hash_10().
+    ::// m_current_power := (m_current_power * m_multiplier) % m_modulo.
+    ::// m_hash := (m_hash + m_string[[{10}]] * m_current_power) % m_modulo.
+    ::// ret_ := [m_current_power, m_hash] |.
+}
+return.
+Defined.
+Sync.
+
+#[returns=ret_]
+Ursus Definition hash_12: UExpression (uint64 * uint64) false.
+{
+    ::// [m_current_power, m_hash] := hash_11().
+    ::// m_current_power := (m_current_power * m_multiplier) % m_modulo.
+    ::// m_hash := (m_hash + m_string[[{11}]] * m_current_power) % m_modulo.
+    ::// ret_ := [m_current_power, m_hash] |.
+}
+return.
+Defined.
+Sync.
+
+#[returns=ret_]
+Ursus Definition hash_13: UExpression (uint64 * uint64) false.
+{
+    ::// [m_current_power, m_hash] := hash_12().
+    ::// m_current_power := (m_current_power * m_multiplier) % m_modulo.
+    ::// m_hash := (m_hash + m_string[[{12}]] * m_current_power) % m_modulo.
+    ::// ret_ := [m_current_power, m_hash] |.
+}
+return.
+Defined.
+Sync.
+
+#[returns=ret_]
+Ursus Definition hash_14: UExpression (uint64 * uint64) false.
+{
+    ::// [m_current_power, m_hash] := hash_13().
+    ::// m_current_power := (m_current_power * m_multiplier) % m_modulo.
+    ::// m_hash := (m_hash + m_string[[{13}]] * m_current_power) % m_modulo.
+    ::// ret_ := [m_current_power, m_hash] |.
+}
+return.
+Defined.
+Sync.
+
+#[returns=ret_]
+Ursus Definition hash_15: UExpression (uint64 * uint64) false.
+{
+    ::// [m_current_power, m_hash] := hash_14().
+    ::// m_current_power := (m_current_power * m_multiplier) % m_modulo.
+    ::// m_hash := (m_hash + m_string[[{14}]] * m_current_power) % m_modulo.
+    ::// ret_ := [m_current_power, m_hash] |.
+}
+return.
+Defined.
+Sync.
+
+#[returns=ret_]
+Ursus Definition hash_16: UExpression (uint64 * uint64) false.
+{
+    ::// [m_current_power, m_hash] := hash_15().
+    ::// m_current_power := (m_current_power * m_multiplier) % m_modulo.
+    ::// m_hash := (m_hash + m_string[[{15}]] * m_current_power) % m_modulo.
+    ::// ret_ := [m_current_power, m_hash] |.
+}
+return.
+Defined.
+Sync.
+
+#[returns=ret_]
+Ursus Definition hash_17: UExpression (uint64 * uint64) false.
+{
+    ::// [m_current_power, m_hash] := hash_16().
+    ::// m_current_power := (m_current_power * m_multiplier) % m_modulo.
+    ::// m_hash := (m_hash + m_string[[{16}]] * m_current_power) % m_modulo.
+    ::// ret_ := [m_current_power, m_hash] |.
+}
+return.
+Defined.
+Sync.
+
+#[returns=ret_]
+Ursus Definition hash_18: UExpression (uint64 * uint64) false.
+{
+    ::// [m_current_power, m_hash] := hash_17().
+    ::// m_current_power := (m_current_power * m_multiplier) % m_modulo.
+    ::// m_hash := (m_hash + m_string[[{17}]] * m_current_power) % m_modulo.
+    ::// ret_ := [m_current_power, m_hash] |.
+}
+return.
+Defined.
+Sync.
+
+#[returns=ret_]
+Ursus Definition hash_19: UExpression (uint64 * uint64) false.
+{
+    ::// [m_current_power, m_hash] := hash_18().
+    ::// m_current_power := (m_current_power * m_multiplier) % m_modulo.
+    ::// m_hash := (m_hash + m_string[[{18}]] * m_current_power) % m_modulo.
+    ::// ret_ := [m_current_power, m_hash] |.
+}
+return.
+Defined.
+Sync.
+
+#[returns=ret_]
+Ursus Definition hash_20: UExpression (uint64 * uint64) false.
+{
+    ::// [m_current_power, m_hash] := hash_19().
+    ::// m_current_power := (m_current_power * m_multiplier) % m_modulo.
+    ::// m_hash := (m_hash + m_string[[{19}]] * m_current_power) % m_modulo.
+    ::// ret_ := [m_current_power, m_hash] |.
+}
+return.
+Defined.
+Sync.
+
+#[returns=ret_]
+Ursus Definition hash_21: UExpression (uint64 * uint64) false.
+{
+    ::// [m_current_power, m_hash] := hash_20().
+    ::// m_current_power := (m_current_power * m_multiplier) % m_modulo.
+    ::// m_hash := (m_hash + m_string[[{20}]] * m_current_power) % m_modulo.
+    ::// ret_ := [m_current_power, m_hash] |.
+}
+return.
+Defined.
+Sync.
+
+#[returns=ret_]
+Ursus Definition hash_22: UExpression (uint64 * uint64) false.
+{
+    ::// [m_current_power, m_hash] := hash_21().
+    ::// m_current_power := (m_current_power * m_multiplier) % m_modulo.
+    ::// m_hash := (m_hash + m_string[[{21}]] * m_current_power) % m_modulo.
+    ::// ret_ := [m_current_power, m_hash] |.
+}
+return.
+Defined.
+Sync.
+
+#[returns=ret_]
+Ursus Definition hash_23: UExpression (uint64 * uint64) false.
+{
+    ::// [m_current_power, m_hash] := hash_22().
+    ::// m_current_power := (m_current_power * m_multiplier) % m_modulo.
+    ::// m_hash := (m_hash + m_string[[{22}]] * m_current_power) % m_modulo.
+    ::// ret_ := [m_current_power, m_hash] |.
+}
+return.
+Defined.
+Sync.
+
+#[returns=ret_]
+Ursus Definition hash_24: UExpression (uint64 * uint64) false.
+{
+    ::// [m_current_power, m_hash] := hash_23().
+    ::// m_current_power := (m_current_power * m_multiplier) % m_modulo.
+    ::// m_hash := (m_hash + m_string[[{23}]] * m_current_power) % m_modulo.
+    ::// ret_ := [m_current_power, m_hash] |.
+}
+return.
+Defined.
+Sync.
+
+#[returns=ret_]
+Ursus Definition hash_25: UExpression (uint64 * uint64) false.
+{
+    ::// [m_current_power, m_hash] := hash_24().
+    ::// m_current_power := (m_current_power * m_multiplier) % m_modulo.
+    ::// m_hash := (m_hash + m_string[[{24}]] * m_current_power) % m_modulo.
+    ::// ret_ := [m_current_power, m_hash] |.
+}
+return.
+Defined.
+Sync.
+
+#[returns=ret_]
+Ursus Definition hash_26: UExpression (uint64 * uint64) false.
+{
+    ::// [m_current_power, m_hash] := hash_25().
+    ::// m_current_power := (m_current_power * m_multiplier) % m_modulo.
+    ::// m_hash := (m_hash + m_string[[{25}]] * m_current_power) % m_modulo.
+    ::// ret_ := [m_current_power, m_hash] |.
+}
+return.
+Defined.
+Sync.
+
+#[returns=ret_]
+Ursus Definition hash_27: UExpression (uint64 * uint64) false.
+{
+    ::// [m_current_power, m_hash] := hash_26().
+    ::// m_current_power := (m_current_power * m_multiplier) % m_modulo.
+    ::// m_hash := (m_hash + m_string[[{26}]] * m_current_power) % m_modulo.
+    ::// ret_ := [m_current_power, m_hash] |.
+}
+return.
+Defined.
+Sync.
+
+#[returns=ret_]
+Ursus Definition hash_28: UExpression (uint64 * uint64) false.
+{
+    ::// [m_current_power, m_hash] := hash_27().
+    ::// m_current_power := (m_current_power * m_multiplier) % m_modulo.
+    ::// m_hash := (m_hash + m_string[[{27}]] * m_current_power) % m_modulo.
+    ::// ret_ := [m_current_power, m_hash] |.
+}
+return.
+Defined.
+Sync.
+
+#[returns=ret_]
+Ursus Definition hash_29: UExpression (uint64 * uint64) false.
+{
+    ::// [m_current_power, m_hash] := hash_28().
+    ::// m_current_power := (m_current_power * m_multiplier) % m_modulo.
+    ::// m_hash := (m_hash + m_string[[{28}]] * m_current_power) % m_modulo.
+    ::// ret_ := [m_current_power, m_hash] |.
+}
+return.
+Defined.
+Sync.
+
+#[returns=ret_]
+Ursus Definition hash_30: UExpression (uint64 * uint64) false.
+{
+    ::// [m_current_power, m_hash] := hash_29().
+    ::// m_current_power := (m_current_power * m_multiplier) % m_modulo.
+    ::// m_hash := (m_hash + m_string[[{29}]] * m_current_power) % m_modulo.
+    ::// ret_ := [m_current_power, m_hash] |.
+}
+return.
+Defined.
+Sync.
+
+#[returns=ret_]
+Ursus Definition hash_31: UExpression (uint64 * uint64) false.
+{
+    ::// [m_current_power, m_hash] := hash_30().
+    ::// m_current_power := (m_current_power * m_multiplier) % m_modulo.
+    ::// m_hash := (m_hash + m_string[[{30}]] * m_current_power) % m_modulo.
+    ::// ret_ := [m_current_power, m_hash] |.
+}
+return.
+Defined.
+Sync.
+
+#[returns=ret_]
+Ursus Definition hash_32: UExpression (uint64 * uint64) false.
+{
+    ::// [m_current_power, m_hash] := hash_31().
+    ::// m_current_power := (m_current_power * m_multiplier) % m_modulo.
+    ::// m_hash := (m_hash + m_string[[{31}]] * m_current_power) % m_modulo.
+    ::// ret_ := [m_current_power, m_hash] |.
+}
+return.
+Defined.
+Sync.
+
+#[returns=ret_]
+Ursus Definition hash_33: UExpression (uint64 * uint64) false.
+{
+    ::// [m_current_power, m_hash] := hash_32().
+    ::// m_current_power := (m_current_power * m_multiplier) % m_modulo.
+    ::// m_hash := (m_hash + m_string[[{32}]] * m_current_power) % m_modulo.
+    ::// ret_ := [m_current_power, m_hash] |.
+}
+return.
+Defined.
+Sync.
+
+#[returns=ret_]
+Ursus Definition hash_34: UExpression (uint64 * uint64) false.
+{
+    ::// [m_current_power, m_hash] := hash_33().
+    ::// m_current_power := (m_current_power * m_multiplier) % m_modulo.
+    ::// m_hash := (m_hash + m_string[[{33}]] * m_current_power) % m_modulo.
+    ::// ret_ := [m_current_power, m_hash] |.
+}
+return.
+Defined.
+Sync.
+
+#[returns=ret_]
+Ursus Definition hash_35: UExpression (uint64 * uint64) false.
+{
+    ::// [m_current_power, m_hash] := hash_34().
+    ::// m_current_power := (m_current_power * m_multiplier) % m_modulo.
+    ::// m_hash := (m_hash + m_string[[{34}]] * m_current_power) % m_modulo.
+    ::// ret_ := [m_current_power, m_hash] |.
+}
+return.
+Defined.
+Sync.
+
+#[returns=ret_]
+Ursus Definition hash_36: UExpression (uint64 * uint64) false.
+{
+    ::// [m_current_power, m_hash] := hash_35().
+    ::// m_current_power := (m_current_power * m_multiplier) % m_modulo.
+    ::// m_hash := (m_hash + m_string[[{35}]] * m_current_power) % m_modulo.
+    ::// ret_ := [m_current_power, m_hash] |.
+}
+return.
+Defined.
+Sync.
+
+#[returns=ret_]
+Ursus Definition hash_37: UExpression (uint64 * uint64) false.
+{
+    ::// [m_current_power, m_hash] := hash_36().
+    ::// m_current_power := (m_current_power * m_multiplier) % m_modulo.
+    ::// m_hash := (m_hash + m_string[[{36}]] * m_current_power) % m_modulo.
+    ::// ret_ := [m_current_power, m_hash] |.
+}
+return.
+Defined.
+Sync.
+
+#[returns=ret_]
+Ursus Definition hash_38: UExpression (uint64 * uint64) false.
+{
+    ::// [m_current_power, m_hash] := hash_37().
+    ::// m_current_power := (m_current_power * m_multiplier) % m_modulo.
+    ::// m_hash := (m_hash + m_string[[{37}]] * m_current_power) % m_modulo.
+    ::// ret_ := [m_current_power, m_hash] |.
+}
+return.
+Defined.
+Sync.
+
+#[returns=ret_]
+Ursus Definition hash_39: UExpression (uint64 * uint64) false.
+{
+    ::// [m_current_power, m_hash] := hash_38().
+    ::// m_current_power := (m_current_power * m_multiplier) % m_modulo.
+    ::// m_hash := (m_hash + m_string[[{38}]] * m_current_power) % m_modulo.
+    ::// ret_ := [m_current_power, m_hash] |.
+}
+return.
+Defined.
+Sync.
+
+#[returns=ret_]
+Ursus Definition hash_40: UExpression (uint64 * uint64) false.
+{
+    ::// [m_current_power, m_hash] := hash_39().
+    ::// m_current_power := (m_current_power * m_multiplier) % m_modulo.
+    ::// m_hash := (m_hash + m_string[[{39}]] * m_current_power) % m_modulo.
     ::// ret_ := [m_current_power, m_hash] |.
 }
 return.
