src/Recursion/Run.v
@@ -32,7 +32,37 @@ Definition roots_eval : Datatypes.list string := [
                                        "hash_7";
                                        "hash_8";
                                        "hash_9";
-                                       "hash_10"
+                                       "hash_10";
+                                       "hash_11";
+                                       "hash_12";
+                                       "hash_13";
+                                       "hash_14";
+                                       "hash_15";
+                                       "hash_16";
+                                       "hash_17";
+                                       "hash_18";
+                                       "hash_19";
+                                       "hash_20";
+                                       "hash_21";
+                                       "hash_22";
+                                       "hash_23";
+                                       "hash_24";
+                                       "hash_25";
+                                       "hash_26";
+                                       "hash_27";
+                                       "hash_28";
+                                       "hash_29";
+                                       "hash_30";
+                                       "hash_31";
+                                       "hash_32";
+                                       "hash_33";
+                                       "hash_34";
+                                       "hash_35";
+                                       "hash_36";
+                                       "hash_37";
+                                       "hash_38";
+                                       "hash_39";
+                                       "hash_40"
 ].
 
 Definition roots_exec : Datatypes.list string := [
@@ -45,7 +75,37 @@ Definition roots_exec : Datatypes.list string := [
                                         "hash_7";
                                         "hash_8";
                                         "hash_9";
-                                        "hash_10"
+                                        "hash_10";
+                                        "hash_11";
+                                        "hash_12";
+                                        "hash_13";
+                                        "hash_14";
+                                        "hash_15";
+                                        "hash_16";
+                                        "hash_17";
+                                        "hash_18";
+                                        "hash_19";
+                                        "hash_20";
+                                        "hash_21";
+                                        "hash_22";
+                                        "hash_23";
+                                        "hash_24";
+                                        "hash_25";
+                                        "hash_26";
+                                        "hash_27";
+                                        "hash_28";
+                                        "hash_29";
+                                        "hash_30";
+                                        "hash_31";
+                                        "hash_32";
+                                        "hash_33";
+                                        "hash_34";
+                                        "hash_35";
+                                        "hash_36";
+                                        "hash_37";
+                                        "hash_38";
+                                        "hash_39";
+                                        "hash_40"                                    
 ].
 
 
