src/Simple/Simple.v
@@ -1440,6 +1440,976 @@ return.
 Defined.
 Sync.
 
+Ursus Definition hash_31: UExpression PhantomType false.
+{
+    ::// var00 current_power: uint64 := {1} ;_|.
+    ::// m_hash := {0} ;_|.
+    |-----------------------------.
+    ::// m_hash := (m_hash + m_string[[{0}]] * current_power) % m_modulo.
+    ::// current_power := (current_power * m_multiplier) % m_modulo.
+    ::// m_hash := (m_hash + m_string[[{1}]] * current_power) % m_modulo.
+    ::// current_power := (current_power * m_multiplier) % m_modulo.
+    |-----------------------------.
+    ::// m_hash := (m_hash + m_string[[{2}]] * current_power) % m_modulo.
+    ::// current_power := (current_power * m_multiplier) % m_modulo.
+    ::// m_hash := (m_hash + m_string[[{3}]] * current_power) % m_modulo.
+    ::// current_power := (current_power * m_multiplier) % m_modulo.
+    |-----------------------------.
+    ::// m_hash := (m_hash + m_string[[{4}]] * current_power) % m_modulo.
+    ::// current_power := (current_power * m_multiplier) % m_modulo.
+    ::// m_hash := (m_hash + m_string[[{5}]] * current_power) % m_modulo.
+    ::// current_power := (current_power * m_multiplier) % m_modulo.
+    |-----------------------------.
+    ::// m_hash := (m_hash + m_string[[{6}]] * current_power) % m_modulo.
+    ::// current_power := (current_power * m_multiplier) % m_modulo.
+    ::// m_hash := (m_hash + m_string[[{7}]] * current_power) % m_modulo.
+    ::// current_power := (current_power * m_multiplier) % m_modulo.
+    |-----------------------------.
+    ::// m_hash := (m_hash + m_string[[{8}]] * current_power) % m_modulo.
+    ::// current_power := (current_power * m_multiplier) % m_modulo.
+    ::// m_hash := (m_hash + m_string[[{9}]] * current_power) % m_modulo.
+    ::// current_power := (current_power * m_multiplier) % m_modulo.
+    |-----------------------------.
+    ::// m_hash := (m_hash + m_string[[{10}]] * current_power) % m_modulo.
+    ::// current_power := (current_power * m_multiplier) % m_modulo.
+    ::// m_hash := (m_hash + m_string[[{11}]] * current_power) % m_modulo.
+    ::// current_power := (current_power * m_multiplier) % m_modulo.
+    |-----------------------------.
+    ::// m_hash := (m_hash + m_string[[{12}]] * current_power) % m_modulo.
+    ::// current_power := (current_power * m_multiplier) % m_modulo.
+    ::// m_hash := (m_hash + m_string[[{13}]] * current_power) % m_modulo.
+    ::// current_power := (current_power * m_multiplier) % m_modulo.
+    |-----------------------------.
+    ::// m_hash := (m_hash + m_string[[{14}]] * current_power) % m_modulo.
+    ::// current_power := (current_power * m_multiplier) % m_modulo.
+    ::// m_hash := (m_hash + m_string[[{15}]] * current_power) % m_modulo.
+    ::// current_power := (current_power * m_multiplier) % m_modulo.
+    |-----------------------------.
+    ::// m_hash := (m_hash + m_string[[{16}]] * current_power) % m_modulo.
+    ::// current_power := (current_power * m_multiplier) % m_modulo.
+    ::// m_hash := (m_hash + m_string[[{17}]] * current_power) % m_modulo.
+    ::// current_power := (current_power * m_multiplier) % m_modulo.
+    |-----------------------------.
+    ::// m_hash := (m_hash + m_string[[{18}]] * current_power) % m_modulo.
+    ::// current_power := (current_power * m_multiplier) % m_modulo.
+    ::// m_hash := (m_hash + m_string[[{19}]] * current_power) % m_modulo.
+    ::// current_power := (current_power * m_multiplier) % m_modulo.
+    |-----------------------------.
+    ::// m_hash := (m_hash + m_string[[{20}]] * current_power) % m_modulo.
+    ::// current_power := (current_power * m_multiplier) % m_modulo.
+    ::// m_hash := (m_hash + m_string[[{21}]] * current_power) % m_modulo.
+    ::// current_power := (current_power * m_multiplier) % m_modulo.
+    |-----------------------------.
+    ::// m_hash := (m_hash + m_string[[{22}]] * current_power) % m_modulo.
+    ::// current_power := (current_power * m_multiplier) % m_modulo.
+    ::// m_hash := (m_hash + m_string[[{23}]] * current_power) % m_modulo.
+    ::// current_power := (current_power * m_multiplier) % m_modulo.
+    |-----------------------------.
+    ::// m_hash := (m_hash + m_string[[{24}]] * current_power) % m_modulo.
+    ::// current_power := (current_power * m_multiplier) % m_modulo.
+    ::// m_hash := (m_hash + m_string[[{25}]] * current_power) % m_modulo.
+    ::// current_power := (current_power * m_multiplier) % m_modulo.
+    |-----------------------------.
+    ::// m_hash := (m_hash + m_string[[{26}]] * current_power) % m_modulo.
+    ::// current_power := (current_power * m_multiplier) % m_modulo.
+    ::// m_hash := (m_hash + m_string[[{27}]] * current_power) % m_modulo.
+    ::// current_power := (current_power * m_multiplier) % m_modulo.
+    |-----------------------------.
+    ::// m_hash := (m_hash + m_string[[{28}]] * current_power) % m_modulo.
+    ::// current_power := (current_power * m_multiplier) % m_modulo.
+    ::// m_hash := (m_hash + m_string[[{29}]] * current_power) % m_modulo.
+    ::// current_power := (current_power * m_multiplier) % m_modulo.
+    |-----------------------------.
+    ::// m_hash := (m_hash + m_string[[{30}]] * current_power) % m_modulo |.
+}
+return.
+Defined.
+Sync.
+
+Ursus Definition hash_32: UExpression PhantomType false.
+{
+    ::// var00 current_power: uint64 := {1} ;_|.
+    ::// m_hash := {0} ;_|.
+    |-----------------------------.
+    ::// m_hash := (m_hash + m_string[[{0}]] * current_power) % m_modulo.
+    ::// current_power := (current_power * m_multiplier) % m_modulo.
+    ::// m_hash := (m_hash + m_string[[{1}]] * current_power) % m_modulo.
+    ::// current_power := (current_power * m_multiplier) % m_modulo.
+    |-----------------------------.
+    ::// m_hash := (m_hash + m_string[[{2}]] * current_power) % m_modulo.
+    ::// current_power := (current_power * m_multiplier) % m_modulo.
+    ::// m_hash := (m_hash + m_string[[{3}]] * current_power) % m_modulo.
+    ::// current_power := (current_power * m_multiplier) % m_modulo.
+    |-----------------------------.
+    ::// m_hash := (m_hash + m_string[[{4}]] * current_power) % m_modulo.
+    ::// current_power := (current_power * m_multiplier) % m_modulo.
+    ::// m_hash := (m_hash + m_string[[{5}]] * current_power) % m_modulo.
+    ::// current_power := (current_power * m_multiplier) % m_modulo.
+    |-----------------------------.
+    ::// m_hash := (m_hash + m_string[[{6}]] * current_power) % m_modulo.
+    ::// current_power := (current_power * m_multiplier) % m_modulo.
+    ::// m_hash := (m_hash + m_string[[{7}]] * current_power) % m_modulo.
+    ::// current_power := (current_power * m_multiplier) % m_modulo.
+    |-----------------------------.
+    ::// m_hash := (m_hash + m_string[[{8}]] * current_power) % m_modulo.
+    ::// current_power := (current_power * m_multiplier) % m_modulo.
+    ::// m_hash := (m_hash + m_string[[{9}]] * current_power) % m_modulo.
+    ::// current_power := (current_power * m_multiplier) % m_modulo.
+    |-----------------------------.
+    ::// m_hash := (m_hash + m_string[[{10}]] * current_power) % m_modulo.
+    ::// current_power := (current_power * m_multiplier) % m_modulo.
+    ::// m_hash := (m_hash + m_string[[{11}]] * current_power) % m_modulo.
+    ::// current_power := (current_power * m_multiplier) % m_modulo.
+    |-----------------------------.
+    ::// m_hash := (m_hash + m_string[[{12}]] * current_power) % m_modulo.
+    ::// current_power := (current_power * m_multiplier) % m_modulo.
+    ::// m_hash := (m_hash + m_string[[{13}]] * current_power) % m_modulo.
+    ::// current_power := (current_power * m_multiplier) % m_modulo.
+    |-----------------------------.
+    ::// m_hash := (m_hash + m_string[[{14}]] * current_power) % m_modulo.
+    ::// current_power := (current_power * m_multiplier) % m_modulo.
+    ::// m_hash := (m_hash + m_string[[{15}]] * current_power) % m_modulo.
+    ::// current_power := (current_power * m_multiplier) % m_modulo.
+    |-----------------------------.
+    ::// m_hash := (m_hash + m_string[[{16}]] * current_power) % m_modulo.
+    ::// current_power := (current_power * m_multiplier) % m_modulo.
+    ::// m_hash := (m_hash + m_string[[{17}]] * current_power) % m_modulo.
+    ::// current_power := (current_power * m_multiplier) % m_modulo.
+    |-----------------------------.
+    ::// m_hash := (m_hash + m_string[[{18}]] * current_power) % m_modulo.
+    ::// current_power := (current_power * m_multiplier) % m_modulo.
+    ::// m_hash := (m_hash + m_string[[{19}]] * current_power) % m_modulo.
+    ::// current_power := (current_power * m_multiplier) % m_modulo.
+    |-----------------------------.
+    ::// m_hash := (m_hash + m_string[[{20}]] * current_power) % m_modulo.
+    ::// current_power := (current_power * m_multiplier) % m_modulo.
+    ::// m_hash := (m_hash + m_string[[{21}]] * current_power) % m_modulo.
+    ::// current_power := (current_power * m_multiplier) % m_modulo.
+    |-----------------------------.
+    ::// m_hash := (m_hash + m_string[[{22}]] * current_power) % m_modulo.
+    ::// current_power := (current_power * m_multiplier) % m_modulo.
+    ::// m_hash := (m_hash + m_string[[{23}]] * current_power) % m_modulo.
+    ::// current_power := (current_power * m_multiplier) % m_modulo.
+    |-----------------------------.
+    ::// m_hash := (m_hash + m_string[[{24}]] * current_power) % m_modulo.
+    ::// current_power := (current_power * m_multiplier) % m_modulo.
+    ::// m_hash := (m_hash + m_string[[{25}]] * current_power) % m_modulo.
+    ::// current_power := (current_power * m_multiplier) % m_modulo.
+    |-----------------------------.
+    ::// m_hash := (m_hash + m_string[[{26}]] * current_power) % m_modulo.
+    ::// current_power := (current_power * m_multiplier) % m_modulo.
+    ::// m_hash := (m_hash + m_string[[{27}]] * current_power) % m_modulo.
+    ::// current_power := (current_power * m_multiplier) % m_modulo.
+    |-----------------------------.
+    ::// m_hash := (m_hash + m_string[[{28}]] * current_power) % m_modulo.
+    ::// current_power := (current_power * m_multiplier) % m_modulo.
+    ::// m_hash := (m_hash + m_string[[{29}]] * current_power) % m_modulo.
+    ::// current_power := (current_power * m_multiplier) % m_modulo.
+    |-----------------------------.
+    ::// m_hash := (m_hash + m_string[[{30}]] * current_power) % m_modulo.
+    ::// current_power := (current_power * m_multiplier) % m_modulo.
+    ::// m_hash := (m_hash + m_string[[{31}]] * current_power) % m_modulo |.
+}
+return.
+Defined.
+Sync.
+
+Ursus Definition hash_33: UExpression PhantomType false.
+{
+    ::// var00 current_power: uint64 := {1} ;_|.
+    ::// m_hash := {0} ;_|.
+    |-----------------------------.
+    ::// m_hash := (m_hash + m_string[[{0}]] * current_power) % m_modulo.
+    ::// current_power := (current_power * m_multiplier) % m_modulo.
+    ::// m_hash := (m_hash + m_string[[{1}]] * current_power) % m_modulo.
+    ::// current_power := (current_power * m_multiplier) % m_modulo.
+    |-----------------------------.
+    ::// m_hash := (m_hash + m_string[[{2}]] * current_power) % m_modulo.
+    ::// current_power := (current_power * m_multiplier) % m_modulo.
+    ::// m_hash := (m_hash + m_string[[{3}]] * current_power) % m_modulo.
+    ::// current_power := (current_power * m_multiplier) % m_modulo.
+    |-----------------------------.
+    ::// m_hash := (m_hash + m_string[[{4}]] * current_power) % m_modulo.
+    ::// current_power := (current_power * m_multiplier) % m_modulo.
+    ::// m_hash := (m_hash + m_string[[{5}]] * current_power) % m_modulo.
+    ::// current_power := (current_power * m_multiplier) % m_modulo.
+    |-----------------------------.
+    ::// m_hash := (m_hash + m_string[[{6}]] * current_power) % m_modulo.
+    ::// current_power := (current_power * m_multiplier) % m_modulo.
+    ::// m_hash := (m_hash + m_string[[{7}]] * current_power) % m_modulo.
+    ::// current_power := (current_power * m_multiplier) % m_modulo.
+    |-----------------------------.
+    ::// m_hash := (m_hash + m_string[[{8}]] * current_power) % m_modulo.
+    ::// current_power := (current_power * m_multiplier) % m_modulo.
+    ::// m_hash := (m_hash + m_string[[{9}]] * current_power) % m_modulo.
+    ::// current_power := (current_power * m_multiplier) % m_modulo.
+    |-----------------------------.
+    ::// m_hash := (m_hash + m_string[[{10}]] * current_power) % m_modulo.
+    ::// current_power := (current_power * m_multiplier) % m_modulo.
+    ::// m_hash := (m_hash + m_string[[{11}]] * current_power) % m_modulo.
+    ::// current_power := (current_power * m_multiplier) % m_modulo.
+    |-----------------------------.
+    ::// m_hash := (m_hash + m_string[[{12}]] * current_power) % m_modulo.
+    ::// current_power := (current_power * m_multiplier) % m_modulo.
+    ::// m_hash := (m_hash + m_string[[{13}]] * current_power) % m_modulo.
+    ::// current_power := (current_power * m_multiplier) % m_modulo.
+    |-----------------------------.
+    ::// m_hash := (m_hash + m_string[[{14}]] * current_power) % m_modulo.
+    ::// current_power := (current_power * m_multiplier) % m_modulo.
+    ::// m_hash := (m_hash + m_string[[{15}]] * current_power) % m_modulo.
+    ::// current_power := (current_power * m_multiplier) % m_modulo.
+    |-----------------------------.
+    ::// m_hash := (m_hash + m_string[[{16}]] * current_power) % m_modulo.
+    ::// current_power := (current_power * m_multiplier) % m_modulo.
+    ::// m_hash := (m_hash + m_string[[{17}]] * current_power) % m_modulo.
+    ::// current_power := (current_power * m_multiplier) % m_modulo.
+    |-----------------------------.
+    ::// m_hash := (m_hash + m_string[[{18}]] * current_power) % m_modulo.
+    ::// current_power := (current_power * m_multiplier) % m_modulo.
+    ::// m_hash := (m_hash + m_string[[{19}]] * current_power) % m_modulo.
+    ::// current_power := (current_power * m_multiplier) % m_modulo.
+    |-----------------------------.
+    ::// m_hash := (m_hash + m_string[[{20}]] * current_power) % m_modulo.
+    ::// current_power := (current_power * m_multiplier) % m_modulo.
+    ::// m_hash := (m_hash + m_string[[{21}]] * current_power) % m_modulo.
+    ::// current_power := (current_power * m_multiplier) % m_modulo.
+    |-----------------------------.
+    ::// m_hash := (m_hash + m_string[[{22}]] * current_power) % m_modulo.
+    ::// current_power := (current_power * m_multiplier) % m_modulo.
+    ::// m_hash := (m_hash + m_string[[{23}]] * current_power) % m_modulo.
+    ::// current_power := (current_power * m_multiplier) % m_modulo.
+    |-----------------------------.
+    ::// m_hash := (m_hash + m_string[[{24}]] * current_power) % m_modulo.
+    ::// current_power := (current_power * m_multiplier) % m_modulo.
+    ::// m_hash := (m_hash + m_string[[{25}]] * current_power) % m_modulo.
+    ::// current_power := (current_power * m_multiplier) % m_modulo.
+    |-----------------------------.
+    ::// m_hash := (m_hash + m_string[[{26}]] * current_power) % m_modulo.
+    ::// current_power := (current_power * m_multiplier) % m_modulo.
+    ::// m_hash := (m_hash + m_string[[{27}]] * current_power) % m_modulo.
+    ::// current_power := (current_power * m_multiplier) % m_modulo.
+    |-----------------------------.
+    ::// m_hash := (m_hash + m_string[[{28}]] * current_power) % m_modulo.
+    ::// current_power := (current_power * m_multiplier) % m_modulo.
+    ::// m_hash := (m_hash + m_string[[{29}]] * current_power) % m_modulo.
+    ::// current_power := (current_power * m_multiplier) % m_modulo.
+    |-----------------------------.
+    ::// m_hash := (m_hash + m_string[[{30}]] * current_power) % m_modulo.
+    ::// current_power := (current_power * m_multiplier) % m_modulo.
+    ::// m_hash := (m_hash + m_string[[{31}]] * current_power) % m_modulo.
+    ::// current_power := (current_power * m_multiplier) % m_modulo.
+    |-----------------------------.
+    ::// m_hash := (m_hash + m_string[[{32}]] * current_power) % m_modulo |.
+}
+return.
+Defined.
+Sync.
+
+Ursus Definition hash_34: UExpression PhantomType false.
+{
+    ::// var00 current_power: uint64 := {1} ;_|.
+    ::// m_hash := {0} ;_|.
+    |-----------------------------.
+    ::// m_hash := (m_hash + m_string[[{0}]] * current_power) % m_modulo.
+    ::// current_power := (current_power * m_multiplier) % m_modulo.
+    ::// m_hash := (m_hash + m_string[[{1}]] * current_power) % m_modulo.
+    ::// current_power := (current_power * m_multiplier) % m_modulo.
+    |-----------------------------.
+    ::// m_hash := (m_hash + m_string[[{2}]] * current_power) % m_modulo.
+    ::// current_power := (current_power * m_multiplier) % m_modulo.
+    ::// m_hash := (m_hash + m_string[[{3}]] * current_power) % m_modulo.
+    ::// current_power := (current_power * m_multiplier) % m_modulo.
+    |-----------------------------.
+    ::// m_hash := (m_hash + m_string[[{4}]] * current_power) % m_modulo.
+    ::// current_power := (current_power * m_multiplier) % m_modulo.
+    ::// m_hash := (m_hash + m_string[[{5}]] * current_power) % m_modulo.
+    ::// current_power := (current_power * m_multiplier) % m_modulo.
+    |-----------------------------.
+    ::// m_hash := (m_hash + m_string[[{6}]] * current_power) % m_modulo.
+    ::// current_power := (current_power * m_multiplier) % m_modulo.
+    ::// m_hash := (m_hash + m_string[[{7}]] * current_power) % m_modulo.
+    ::// current_power := (current_power * m_multiplier) % m_modulo.
+    |-----------------------------.
+    ::// m_hash := (m_hash + m_string[[{8}]] * current_power) % m_modulo.
+    ::// current_power := (current_power * m_multiplier) % m_modulo.
+    ::// m_hash := (m_hash + m_string[[{9}]] * current_power) % m_modulo.
+    ::// current_power := (current_power * m_multiplier) % m_modulo.
+    |-----------------------------.
+    ::// m_hash := (m_hash + m_string[[{10}]] * current_power) % m_modulo.
+    ::// current_power := (current_power * m_multiplier) % m_modulo.
+    ::// m_hash := (m_hash + m_string[[{11}]] * current_power) % m_modulo.
+    ::// current_power := (current_power * m_multiplier) % m_modulo.
+    |-----------------------------.
+    ::// m_hash := (m_hash + m_string[[{12}]] * current_power) % m_modulo.
+    ::// current_power := (current_power * m_multiplier) % m_modulo.
+    ::// m_hash := (m_hash + m_string[[{13}]] * current_power) % m_modulo.
+    ::// current_power := (current_power * m_multiplier) % m_modulo.
+    |-----------------------------.
+    ::// m_hash := (m_hash + m_string[[{14}]] * current_power) % m_modulo.
+    ::// current_power := (current_power * m_multiplier) % m_modulo.
+    ::// m_hash := (m_hash + m_string[[{15}]] * current_power) % m_modulo.
+    ::// current_power := (current_power * m_multiplier) % m_modulo.
+    |-----------------------------.
+    ::// m_hash := (m_hash + m_string[[{16}]] * current_power) % m_modulo.
+    ::// current_power := (current_power * m_multiplier) % m_modulo.
+    ::// m_hash := (m_hash + m_string[[{17}]] * current_power) % m_modulo.
+    ::// current_power := (current_power * m_multiplier) % m_modulo.
+    |-----------------------------.
+    ::// m_hash := (m_hash + m_string[[{18}]] * current_power) % m_modulo.
+    ::// current_power := (current_power * m_multiplier) % m_modulo.
+    ::// m_hash := (m_hash + m_string[[{19}]] * current_power) % m_modulo.
+    ::// current_power := (current_power * m_multiplier) % m_modulo.
+    |-----------------------------.
+    ::// m_hash := (m_hash + m_string[[{20}]] * current_power) % m_modulo.
+    ::// current_power := (current_power * m_multiplier) % m_modulo.
+    ::// m_hash := (m_hash + m_string[[{21}]] * current_power) % m_modulo.
+    ::// current_power := (current_power * m_multiplier) % m_modulo.
+    |-----------------------------.
+    ::// m_hash := (m_hash + m_string[[{22}]] * current_power) % m_modulo.
+    ::// current_power := (current_power * m_multiplier) % m_modulo.
+    ::// m_hash := (m_hash + m_string[[{23}]] * current_power) % m_modulo.
+    ::// current_power := (current_power * m_multiplier) % m_modulo.
+    |-----------------------------.
+    ::// m_hash := (m_hash + m_string[[{24}]] * current_power) % m_modulo.
+    ::// current_power := (current_power * m_multiplier) % m_modulo.
+    ::// m_hash := (m_hash + m_string[[{25}]] * current_power) % m_modulo.
+    ::// current_power := (current_power * m_multiplier) % m_modulo.
+    |-----------------------------.
+    ::// m_hash := (m_hash + m_string[[{26}]] * current_power) % m_modulo.
+    ::// current_power := (current_power * m_multiplier) % m_modulo.
+    ::// m_hash := (m_hash + m_string[[{27}]] * current_power) % m_modulo.
+    ::// current_power := (current_power * m_multiplier) % m_modulo.
+    |-----------------------------.
+    ::// m_hash := (m_hash + m_string[[{28}]] * current_power) % m_modulo.
+    ::// current_power := (current_power * m_multiplier) % m_modulo.
+    ::// m_hash := (m_hash + m_string[[{29}]] * current_power) % m_modulo.
+    ::// current_power := (current_power * m_multiplier) % m_modulo.
+    |-----------------------------.
+    ::// m_hash := (m_hash + m_string[[{30}]] * current_power) % m_modulo.
+    ::// current_power := (current_power * m_multiplier) % m_modulo.
+    ::// m_hash := (m_hash + m_string[[{31}]] * current_power) % m_modulo.
+    ::// current_power := (current_power * m_multiplier) % m_modulo.
+    |-----------------------------.
+    ::// m_hash := (m_hash + m_string[[{32}]] * current_power) % m_modulo.
+    ::// current_power := (current_power * m_multiplier) % m_modulo.
+    ::// m_hash := (m_hash + m_string[[{33}]] * current_power) % m_modulo |.
+}
+return.
+Defined.
+Sync.
+
+Ursus Definition hash_35: UExpression PhantomType false.
+{
+    ::// var00 current_power: uint64 := {1} ;_|.
+    ::// m_hash := {0} ;_|.
+    |-----------------------------.
+    ::// m_hash := (m_hash + m_string[[{0}]] * current_power) % m_modulo.
+    ::// current_power := (current_power * m_multiplier) % m_modulo.
+    ::// m_hash := (m_hash + m_string[[{1}]] * current_power) % m_modulo.
+    ::// current_power := (current_power * m_multiplier) % m_modulo.
+    |-----------------------------.
+    ::// m_hash := (m_hash + m_string[[{2}]] * current_power) % m_modulo.
+    ::// current_power := (current_power * m_multiplier) % m_modulo.
+    ::// m_hash := (m_hash + m_string[[{3}]] * current_power) % m_modulo.
+    ::// current_power := (current_power * m_multiplier) % m_modulo.
+    |-----------------------------.
+    ::// m_hash := (m_hash + m_string[[{4}]] * current_power) % m_modulo.
+    ::// current_power := (current_power * m_multiplier) % m_modulo.
+    ::// m_hash := (m_hash + m_string[[{5}]] * current_power) % m_modulo.
+    ::// current_power := (current_power * m_multiplier) % m_modulo.
+    |-----------------------------.
+    ::// m_hash := (m_hash + m_string[[{6}]] * current_power) % m_modulo.
+    ::// current_power := (current_power * m_multiplier) % m_modulo.
+    ::// m_hash := (m_hash + m_string[[{7}]] * current_power) % m_modulo.
+    ::// current_power := (current_power * m_multiplier) % m_modulo.
+    |-----------------------------.
+    ::// m_hash := (m_hash + m_string[[{8}]] * current_power) % m_modulo.
+    ::// current_power := (current_power * m_multiplier) % m_modulo.
+    ::// m_hash := (m_hash + m_string[[{9}]] * current_power) % m_modulo.
+    ::// current_power := (current_power * m_multiplier) % m_modulo.
+    |-----------------------------.
+    ::// m_hash := (m_hash + m_string[[{10}]] * current_power) % m_modulo.
+    ::// current_power := (current_power * m_multiplier) % m_modulo.
+    ::// m_hash := (m_hash + m_string[[{11}]] * current_power) % m_modulo.
+    ::// current_power := (current_power * m_multiplier) % m_modulo.
+    |-----------------------------.
+    ::// m_hash := (m_hash + m_string[[{12}]] * current_power) % m_modulo.
+    ::// current_power := (current_power * m_multiplier) % m_modulo.
+    ::// m_hash := (m_hash + m_string[[{13}]] * current_power) % m_modulo.
+    ::// current_power := (current_power * m_multiplier) % m_modulo.
+    |-----------------------------.
+    ::// m_hash := (m_hash + m_string[[{14}]] * current_power) % m_modulo.
+    ::// current_power := (current_power * m_multiplier) % m_modulo.
+    ::// m_hash := (m_hash + m_string[[{15}]] * current_power) % m_modulo.
+    ::// current_power := (current_power * m_multiplier) % m_modulo.
+    |-----------------------------.
+    ::// m_hash := (m_hash + m_string[[{16}]] * current_power) % m_modulo.
+    ::// current_power := (current_power * m_multiplier) % m_modulo.
+    ::// m_hash := (m_hash + m_string[[{17}]] * current_power) % m_modulo.
+    ::// current_power := (current_power * m_multiplier) % m_modulo.
+    |-----------------------------.
+    ::// m_hash := (m_hash + m_string[[{18}]] * current_power) % m_modulo.
+    ::// current_power := (current_power * m_multiplier) % m_modulo.
+    ::// m_hash := (m_hash + m_string[[{19}]] * current_power) % m_modulo.
+    ::// current_power := (current_power * m_multiplier) % m_modulo.
+    |-----------------------------.
+    ::// m_hash := (m_hash + m_string[[{20}]] * current_power) % m_modulo.
+    ::// current_power := (current_power * m_multiplier) % m_modulo.
+    ::// m_hash := (m_hash + m_string[[{21}]] * current_power) % m_modulo.
+    ::// current_power := (current_power * m_multiplier) % m_modulo.
+    |-----------------------------.
+    ::// m_hash := (m_hash + m_string[[{22}]] * current_power) % m_modulo.
+    ::// current_power := (current_power * m_multiplier) % m_modulo.
+    ::// m_hash := (m_hash + m_string[[{23}]] * current_power) % m_modulo.
+    ::// current_power := (current_power * m_multiplier) % m_modulo.
+    |-----------------------------.
+    ::// m_hash := (m_hash + m_string[[{24}]] * current_power) % m_modulo.
+    ::// current_power := (current_power * m_multiplier) % m_modulo.
+    ::// m_hash := (m_hash + m_string[[{25}]] * current_power) % m_modulo.
+    ::// current_power := (current_power * m_multiplier) % m_modulo.
+    |-----------------------------.
+    ::// m_hash := (m_hash + m_string[[{26}]] * current_power) % m_modulo.
+    ::// current_power := (current_power * m_multiplier) % m_modulo.
+    ::// m_hash := (m_hash + m_string[[{27}]] * current_power) % m_modulo.
+    ::// current_power := (current_power * m_multiplier) % m_modulo.
+    |-----------------------------.
+    ::// m_hash := (m_hash + m_string[[{28}]] * current_power) % m_modulo.
+    ::// current_power := (current_power * m_multiplier) % m_modulo.
+    ::// m_hash := (m_hash + m_string[[{29}]] * current_power) % m_modulo.
+    ::// current_power := (current_power * m_multiplier) % m_modulo.
+    |-----------------------------.
+    ::// m_hash := (m_hash + m_string[[{30}]] * current_power) % m_modulo.
+    ::// current_power := (current_power * m_multiplier) % m_modulo.
+    ::// m_hash := (m_hash + m_string[[{31}]] * current_power) % m_modulo.
+    ::// current_power := (current_power * m_multiplier) % m_modulo.
+    |-----------------------------.
+    ::// m_hash := (m_hash + m_string[[{32}]] * current_power) % m_modulo.
+    ::// current_power := (current_power * m_multiplier) % m_modulo.
+    ::// m_hash := (m_hash + m_string[[{33}]] * current_power) % m_modulo.
+    ::// current_power := (current_power * m_multiplier) % m_modulo.
+    |-----------------------------.
+    ::// m_hash := (m_hash + m_string[[{34}]] * current_power) % m_modulo |.
+}
+return.
+Defined.
+Sync.
+
+Ursus Definition hash_36: UExpression PhantomType false.
+{
+    ::// var00 current_power: uint64 := {1} ;_|.
+    ::// m_hash := {0} ;_|.
+    |-----------------------------.
+    ::// m_hash := (m_hash + m_string[[{0}]] * current_power) % m_modulo.
+    ::// current_power := (current_power * m_multiplier) % m_modulo.
+    ::// m_hash := (m_hash + m_string[[{1}]] * current_power) % m_modulo.
+    ::// current_power := (current_power * m_multiplier) % m_modulo.
+    |-----------------------------.
+    ::// m_hash := (m_hash + m_string[[{2}]] * current_power) % m_modulo.
+    ::// current_power := (current_power * m_multiplier) % m_modulo.
+    ::// m_hash := (m_hash + m_string[[{3}]] * current_power) % m_modulo.
+    ::// current_power := (current_power * m_multiplier) % m_modulo.
+    |-----------------------------.
+    ::// m_hash := (m_hash + m_string[[{4}]] * current_power) % m_modulo.
+    ::// current_power := (current_power * m_multiplier) % m_modulo.
+    ::// m_hash := (m_hash + m_string[[{5}]] * current_power) % m_modulo.
+    ::// current_power := (current_power * m_multiplier) % m_modulo.
+    |-----------------------------.
+    ::// m_hash := (m_hash + m_string[[{6}]] * current_power) % m_modulo.
+    ::// current_power := (current_power * m_multiplier) % m_modulo.
+    ::// m_hash := (m_hash + m_string[[{7}]] * current_power) % m_modulo.
+    ::// current_power := (current_power * m_multiplier) % m_modulo.
+    |-----------------------------.
+    ::// m_hash := (m_hash + m_string[[{8}]] * current_power) % m_modulo.
+    ::// current_power := (current_power * m_multiplier) % m_modulo.
+    ::// m_hash := (m_hash + m_string[[{9}]] * current_power) % m_modulo.
+    ::// current_power := (current_power * m_multiplier) % m_modulo.
+    |-----------------------------.
+    ::// m_hash := (m_hash + m_string[[{10}]] * current_power) % m_modulo.
+    ::// current_power := (current_power * m_multiplier) % m_modulo.
+    ::// m_hash := (m_hash + m_string[[{11}]] * current_power) % m_modulo.
+    ::// current_power := (current_power * m_multiplier) % m_modulo.
+    |-----------------------------.
+    ::// m_hash := (m_hash + m_string[[{12}]] * current_power) % m_modulo.
+    ::// current_power := (current_power * m_multiplier) % m_modulo.
+    ::// m_hash := (m_hash + m_string[[{13}]] * current_power) % m_modulo.
+    ::// current_power := (current_power * m_multiplier) % m_modulo.
+    |-----------------------------.
+    ::// m_hash := (m_hash + m_string[[{14}]] * current_power) % m_modulo.
+    ::// current_power := (current_power * m_multiplier) % m_modulo.
+    ::// m_hash := (m_hash + m_string[[{15}]] * current_power) % m_modulo.
+    ::// current_power := (current_power * m_multiplier) % m_modulo.
+    |-----------------------------.
+    ::// m_hash := (m_hash + m_string[[{16}]] * current_power) % m_modulo.
+    ::// current_power := (current_power * m_multiplier) % m_modulo.
+    ::// m_hash := (m_hash + m_string[[{17}]] * current_power) % m_modulo.
+    ::// current_power := (current_power * m_multiplier) % m_modulo.
+    |-----------------------------.
+    ::// m_hash := (m_hash + m_string[[{18}]] * current_power) % m_modulo.
+    ::// current_power := (current_power * m_multiplier) % m_modulo.
+    ::// m_hash := (m_hash + m_string[[{19}]] * current_power) % m_modulo.
+    ::// current_power := (current_power * m_multiplier) % m_modulo.
+    |-----------------------------.
+    ::// m_hash := (m_hash + m_string[[{20}]] * current_power) % m_modulo.
+    ::// current_power := (current_power * m_multiplier) % m_modulo.
+    ::// m_hash := (m_hash + m_string[[{21}]] * current_power) % m_modulo.
+    ::// current_power := (current_power * m_multiplier) % m_modulo.
+    |-----------------------------.
+    ::// m_hash := (m_hash + m_string[[{22}]] * current_power) % m_modulo.
+    ::// current_power := (current_power * m_multiplier) % m_modulo.
+    ::// m_hash := (m_hash + m_string[[{23}]] * current_power) % m_modulo.
+    ::// current_power := (current_power * m_multiplier) % m_modulo.
+    |-----------------------------.
+    ::// m_hash := (m_hash + m_string[[{24}]] * current_power) % m_modulo.
+    ::// current_power := (current_power * m_multiplier) % m_modulo.
+    ::// m_hash := (m_hash + m_string[[{25}]] * current_power) % m_modulo.
+    ::// current_power := (current_power * m_multiplier) % m_modulo.
+    |-----------------------------.
+    ::// m_hash := (m_hash + m_string[[{26}]] * current_power) % m_modulo.
+    ::// current_power := (current_power * m_multiplier) % m_modulo.
+    ::// m_hash := (m_hash + m_string[[{27}]] * current_power) % m_modulo.
+    ::// current_power := (current_power * m_multiplier) % m_modulo.
+    |-----------------------------.
+    ::// m_hash := (m_hash + m_string[[{28}]] * current_power) % m_modulo.
+    ::// current_power := (current_power * m_multiplier) % m_modulo.
+    ::// m_hash := (m_hash + m_string[[{29}]] * current_power) % m_modulo.
+    ::// current_power := (current_power * m_multiplier) % m_modulo.
+    |-----------------------------.
+    ::// m_hash := (m_hash + m_string[[{30}]] * current_power) % m_modulo.
+    ::// current_power := (current_power * m_multiplier) % m_modulo.
+    ::// m_hash := (m_hash + m_string[[{31}]] * current_power) % m_modulo.
+    ::// current_power := (current_power * m_multiplier) % m_modulo.
+    |-----------------------------.
+    ::// m_hash := (m_hash + m_string[[{32}]] * current_power) % m_modulo.
+    ::// current_power := (current_power * m_multiplier) % m_modulo.
+    ::// m_hash := (m_hash + m_string[[{33}]] * current_power) % m_modulo.
+    ::// current_power := (current_power * m_multiplier) % m_modulo.
+    |-----------------------------.
+    ::// m_hash := (m_hash + m_string[[{34}]] * current_power) % m_modulo.
+    ::// current_power := (current_power * m_multiplier) % m_modulo.
+    ::// m_hash := (m_hash + m_string[[{35}]] * current_power) % m_modulo |.
+}
+return.
+Defined.
+Sync.
+
+Ursus Definition hash_37: UExpression PhantomType false.
+{
+    ::// var00 current_power: uint64 := {1} ;_|.
+    ::// m_hash := {0} ;_|.
+    |-----------------------------.
+    ::// m_hash := (m_hash + m_string[[{0}]] * current_power) % m_modulo.
+    ::// current_power := (current_power * m_multiplier) % m_modulo.
+    ::// m_hash := (m_hash + m_string[[{1}]] * current_power) % m_modulo.
+    ::// current_power := (current_power * m_multiplier) % m_modulo.
+    |-----------------------------.
+    ::// m_hash := (m_hash + m_string[[{2}]] * current_power) % m_modulo.
+    ::// current_power := (current_power * m_multiplier) % m_modulo.
+    ::// m_hash := (m_hash + m_string[[{3}]] * current_power) % m_modulo.
+    ::// current_power := (current_power * m_multiplier) % m_modulo.
+    |-----------------------------.
+    ::// m_hash := (m_hash + m_string[[{4}]] * current_power) % m_modulo.
+    ::// current_power := (current_power * m_multiplier) % m_modulo.
+    ::// m_hash := (m_hash + m_string[[{5}]] * current_power) % m_modulo.
+    ::// current_power := (current_power * m_multiplier) % m_modulo.
+    |-----------------------------.
+    ::// m_hash := (m_hash + m_string[[{6}]] * current_power) % m_modulo.
+    ::// current_power := (current_power * m_multiplier) % m_modulo.
+    ::// m_hash := (m_hash + m_string[[{7}]] * current_power) % m_modulo.
+    ::// current_power := (current_power * m_multiplier) % m_modulo.
+    |-----------------------------.
+    ::// m_hash := (m_hash + m_string[[{8}]] * current_power) % m_modulo.
+    ::// current_power := (current_power * m_multiplier) % m_modulo.
+    ::// m_hash := (m_hash + m_string[[{9}]] * current_power) % m_modulo.
+    ::// current_power := (current_power * m_multiplier) % m_modulo.
+    |-----------------------------.
+    ::// m_hash := (m_hash + m_string[[{10}]] * current_power) % m_modulo.
+    ::// current_power := (current_power * m_multiplier) % m_modulo.
+    ::// m_hash := (m_hash + m_string[[{11}]] * current_power) % m_modulo.
+    ::// current_power := (current_power * m_multiplier) % m_modulo.
+    |-----------------------------.
+    ::// m_hash := (m_hash + m_string[[{12}]] * current_power) % m_modulo.
+    ::// current_power := (current_power * m_multiplier) % m_modulo.
+    ::// m_hash := (m_hash + m_string[[{13}]] * current_power) % m_modulo.
+    ::// current_power := (current_power * m_multiplier) % m_modulo.
+    |-----------------------------.
+    ::// m_hash := (m_hash + m_string[[{14}]] * current_power) % m_modulo.
+    ::// current_power := (current_power * m_multiplier) % m_modulo.
+    ::// m_hash := (m_hash + m_string[[{15}]] * current_power) % m_modulo.
+    ::// current_power := (current_power * m_multiplier) % m_modulo.
+    |-----------------------------.
+    ::// m_hash := (m_hash + m_string[[{16}]] * current_power) % m_modulo.
+    ::// current_power := (current_power * m_multiplier) % m_modulo.
+    ::// m_hash := (m_hash + m_string[[{17}]] * current_power) % m_modulo.
+    ::// current_power := (current_power * m_multiplier) % m_modulo.
+    |-----------------------------.
+    ::// m_hash := (m_hash + m_string[[{18}]] * current_power) % m_modulo.
+    ::// current_power := (current_power * m_multiplier) % m_modulo.
+    ::// m_hash := (m_hash + m_string[[{19}]] * current_power) % m_modulo.
+    ::// current_power := (current_power * m_multiplier) % m_modulo.
+    |-----------------------------.
+    ::// m_hash := (m_hash + m_string[[{20}]] * current_power) % m_modulo.
+    ::// current_power := (current_power * m_multiplier) % m_modulo.
+    ::// m_hash := (m_hash + m_string[[{21}]] * current_power) % m_modulo.
+    ::// current_power := (current_power * m_multiplier) % m_modulo.
+    |-----------------------------.
+    ::// m_hash := (m_hash + m_string[[{22}]] * current_power) % m_modulo.
+    ::// current_power := (current_power * m_multiplier) % m_modulo.
+    ::// m_hash := (m_hash + m_string[[{23}]] * current_power) % m_modulo.
+    ::// current_power := (current_power * m_multiplier) % m_modulo.
+    |-----------------------------.
+    ::// m_hash := (m_hash + m_string[[{24}]] * current_power) % m_modulo.
+    ::// current_power := (current_power * m_multiplier) % m_modulo.
+    ::// m_hash := (m_hash + m_string[[{25}]] * current_power) % m_modulo.
+    ::// current_power := (current_power * m_multiplier) % m_modulo.
+    |-----------------------------.
+    ::// m_hash := (m_hash + m_string[[{26}]] * current_power) % m_modulo.
+    ::// current_power := (current_power * m_multiplier) % m_modulo.
+    ::// m_hash := (m_hash + m_string[[{27}]] * current_power) % m_modulo.
+    ::// current_power := (current_power * m_multiplier) % m_modulo.
+    |-----------------------------.
+    ::// m_hash := (m_hash + m_string[[{28}]] * current_power) % m_modulo.
+    ::// current_power := (current_power * m_multiplier) % m_modulo.
+    ::// m_hash := (m_hash + m_string[[{29}]] * current_power) % m_modulo.
+    ::// current_power := (current_power * m_multiplier) % m_modulo.
+    |-----------------------------.
+    ::// m_hash := (m_hash + m_string[[{30}]] * current_power) % m_modulo.
+    ::// current_power := (current_power * m_multiplier) % m_modulo.
+    ::// m_hash := (m_hash + m_string[[{31}]] * current_power) % m_modulo.
+    ::// current_power := (current_power * m_multiplier) % m_modulo.
+    |-----------------------------.
+    ::// m_hash := (m_hash + m_string[[{32}]] * current_power) % m_modulo.
+    ::// current_power := (current_power * m_multiplier) % m_modulo.
+    ::// m_hash := (m_hash + m_string[[{33}]] * current_power) % m_modulo.
+    ::// current_power := (current_power * m_multiplier) % m_modulo.
+    |-----------------------------.
+    ::// m_hash := (m_hash + m_string[[{34}]] * current_power) % m_modulo.
+    ::// current_power := (current_power * m_multiplier) % m_modulo.
+    ::// m_hash := (m_hash + m_string[[{35}]] * current_power) % m_modulo.
+    ::// current_power := (current_power * m_multiplier) % m_modulo.
+    |-----------------------------.
+    ::// m_hash := (m_hash + m_string[[{36}]] * current_power) % m_modulo |.
+}
+return.
+Defined.
+Sync.
+
+Ursus Definition hash_38: UExpression PhantomType false.
+{
+    ::// var00 current_power: uint64 := {1} ;_|.
+    ::// m_hash := {0} ;_|.
+    |-----------------------------.
+    ::// m_hash := (m_hash + m_string[[{0}]] * current_power) % m_modulo.
+    ::// current_power := (current_power * m_multiplier) % m_modulo.
+    ::// m_hash := (m_hash + m_string[[{1}]] * current_power) % m_modulo.
+    ::// current_power := (current_power * m_multiplier) % m_modulo.
+    |-----------------------------.
+    ::// m_hash := (m_hash + m_string[[{2}]] * current_power) % m_modulo.
+    ::// current_power := (current_power * m_multiplier) % m_modulo.
+    ::// m_hash := (m_hash + m_string[[{3}]] * current_power) % m_modulo.
+    ::// current_power := (current_power * m_multiplier) % m_modulo.
+    |-----------------------------.
+    ::// m_hash := (m_hash + m_string[[{4}]] * current_power) % m_modulo.
+    ::// current_power := (current_power * m_multiplier) % m_modulo.
+    ::// m_hash := (m_hash + m_string[[{5}]] * current_power) % m_modulo.
+    ::// current_power := (current_power * m_multiplier) % m_modulo.
+    |-----------------------------.
+    ::// m_hash := (m_hash + m_string[[{6}]] * current_power) % m_modulo.
+    ::// current_power := (current_power * m_multiplier) % m_modulo.
+    ::// m_hash := (m_hash + m_string[[{7}]] * current_power) % m_modulo.
+    ::// current_power := (current_power * m_multiplier) % m_modulo.
+    |-----------------------------.
+    ::// m_hash := (m_hash + m_string[[{8}]] * current_power) % m_modulo.
+    ::// current_power := (current_power * m_multiplier) % m_modulo.
+    ::// m_hash := (m_hash + m_string[[{9}]] * current_power) % m_modulo.
+    ::// current_power := (current_power * m_multiplier) % m_modulo.
+    |-----------------------------.
+    ::// m_hash := (m_hash + m_string[[{10}]] * current_power) % m_modulo.
+    ::// current_power := (current_power * m_multiplier) % m_modulo.
+    ::// m_hash := (m_hash + m_string[[{11}]] * current_power) % m_modulo.
+    ::// current_power := (current_power * m_multiplier) % m_modulo.
+    |-----------------------------.
+    ::// m_hash := (m_hash + m_string[[{12}]] * current_power) % m_modulo.
+    ::// current_power := (current_power * m_multiplier) % m_modulo.
+    ::// m_hash := (m_hash + m_string[[{13}]] * current_power) % m_modulo.
+    ::// current_power := (current_power * m_multiplier) % m_modulo.
+    |-----------------------------.
+    ::// m_hash := (m_hash + m_string[[{14}]] * current_power) % m_modulo.
+    ::// current_power := (current_power * m_multiplier) % m_modulo.
+    ::// m_hash := (m_hash + m_string[[{15}]] * current_power) % m_modulo.
+    ::// current_power := (current_power * m_multiplier) % m_modulo.
+    |-----------------------------.
+    ::// m_hash := (m_hash + m_string[[{16}]] * current_power) % m_modulo.
+    ::// current_power := (current_power * m_multiplier) % m_modulo.
+    ::// m_hash := (m_hash + m_string[[{17}]] * current_power) % m_modulo.
+    ::// current_power := (current_power * m_multiplier) % m_modulo.
+    |-----------------------------.
+    ::// m_hash := (m_hash + m_string[[{18}]] * current_power) % m_modulo.
+    ::// current_power := (current_power * m_multiplier) % m_modulo.
+    ::// m_hash := (m_hash + m_string[[{19}]] * current_power) % m_modulo.
+    ::// current_power := (current_power * m_multiplier) % m_modulo.
+    |-----------------------------.
+    ::// m_hash := (m_hash + m_string[[{20}]] * current_power) % m_modulo.
+    ::// current_power := (current_power * m_multiplier) % m_modulo.
+    ::// m_hash := (m_hash + m_string[[{21}]] * current_power) % m_modulo.
+    ::// current_power := (current_power * m_multiplier) % m_modulo.
+    |-----------------------------.
+    ::// m_hash := (m_hash + m_string[[{22}]] * current_power) % m_modulo.
+    ::// current_power := (current_power * m_multiplier) % m_modulo.
+    ::// m_hash := (m_hash + m_string[[{23}]] * current_power) % m_modulo.
+    ::// current_power := (current_power * m_multiplier) % m_modulo.
+    |-----------------------------.
+    ::// m_hash := (m_hash + m_string[[{24}]] * current_power) % m_modulo.
+    ::// current_power := (current_power * m_multiplier) % m_modulo.
+    ::// m_hash := (m_hash + m_string[[{25}]] * current_power) % m_modulo.
+    ::// current_power := (current_power * m_multiplier) % m_modulo.
+    |-----------------------------.
+    ::// m_hash := (m_hash + m_string[[{26}]] * current_power) % m_modulo.
+    ::// current_power := (current_power * m_multiplier) % m_modulo.
+    ::// m_hash := (m_hash + m_string[[{27}]] * current_power) % m_modulo.
+    ::// current_power := (current_power * m_multiplier) % m_modulo.
+    |-----------------------------.
+    ::// m_hash := (m_hash + m_string[[{28}]] * current_power) % m_modulo.
+    ::// current_power := (current_power * m_multiplier) % m_modulo.
+    ::// m_hash := (m_hash + m_string[[{29}]] * current_power) % m_modulo.
+    ::// current_power := (current_power * m_multiplier) % m_modulo.
+    |-----------------------------.
+    ::// m_hash := (m_hash + m_string[[{30}]] * current_power) % m_modulo.
+    ::// current_power := (current_power * m_multiplier) % m_modulo.
+    ::// m_hash := (m_hash + m_string[[{31}]] * current_power) % m_modulo.
+    ::// current_power := (current_power * m_multiplier) % m_modulo.
+    |-----------------------------.
+    ::// m_hash := (m_hash + m_string[[{32}]] * current_power) % m_modulo.
+    ::// current_power := (current_power * m_multiplier) % m_modulo.
+    ::// m_hash := (m_hash + m_string[[{33}]] * current_power) % m_modulo.
+    ::// current_power := (current_power * m_multiplier) % m_modulo.
+    |-----------------------------.
+    ::// m_hash := (m_hash + m_string[[{34}]] * current_power) % m_modulo.
+    ::// current_power := (current_power * m_multiplier) % m_modulo.
+    ::// m_hash := (m_hash + m_string[[{35}]] * current_power) % m_modulo.
+    ::// current_power := (current_power * m_multiplier) % m_modulo.
+    |-----------------------------.
+    ::// m_hash := (m_hash + m_string[[{36}]] * current_power) % m_modulo.
+    ::// current_power := (current_power * m_multiplier) % m_modulo.
+    ::// m_hash := (m_hash + m_string[[{37}]] * current_power) % m_modulo |.
+}
+return.
+Defined.
+Sync.
+
+Ursus Definition hash_39: UExpression PhantomType false.
+{
+    ::// var00 current_power: uint64 := {1} ;_|.
+    ::// m_hash := {0} ;_|.
+    |-----------------------------.
+    ::// m_hash := (m_hash + m_string[[{0}]] * current_power) % m_modulo.
+    ::// current_power := (current_power * m_multiplier) % m_modulo.
+    ::// m_hash := (m_hash + m_string[[{1}]] * current_power) % m_modulo.
+    ::// current_power := (current_power * m_multiplier) % m_modulo.
+    |-----------------------------.
+    ::// m_hash := (m_hash + m_string[[{2}]] * current_power) % m_modulo.
+    ::// current_power := (current_power * m_multiplier) % m_modulo.
+    ::// m_hash := (m_hash + m_string[[{3}]] * current_power) % m_modulo.
+    ::// current_power := (current_power * m_multiplier) % m_modulo.
+    |-----------------------------.
+    ::// m_hash := (m_hash + m_string[[{4}]] * current_power) % m_modulo.
+    ::// current_power := (current_power * m_multiplier) % m_modulo.
+    ::// m_hash := (m_hash + m_string[[{5}]] * current_power) % m_modulo.
+    ::// current_power := (current_power * m_multiplier) % m_modulo.
+    |-----------------------------.
+    ::// m_hash := (m_hash + m_string[[{6}]] * current_power) % m_modulo.
+    ::// current_power := (current_power * m_multiplier) % m_modulo.
+    ::// m_hash := (m_hash + m_string[[{7}]] * current_power) % m_modulo.
+    ::// current_power := (current_power * m_multiplier) % m_modulo.
+    |-----------------------------.
+    ::// m_hash := (m_hash + m_string[[{8}]] * current_power) % m_modulo.
+    ::// current_power := (current_power * m_multiplier) % m_modulo.
+    ::// m_hash := (m_hash + m_string[[{9}]] * current_power) % m_modulo.
+    ::// current_power := (current_power * m_multiplier) % m_modulo.
+    |-----------------------------.
+    ::// m_hash := (m_hash + m_string[[{10}]] * current_power) % m_modulo.
+    ::// current_power := (current_power * m_multiplier) % m_modulo.
+    ::// m_hash := (m_hash + m_string[[{11}]] * current_power) % m_modulo.
+    ::// current_power := (current_power * m_multiplier) % m_modulo.
+    |-----------------------------.
+    ::// m_hash := (m_hash + m_string[[{12}]] * current_power) % m_modulo.
+    ::// current_power := (current_power * m_multiplier) % m_modulo.
+    ::// m_hash := (m_hash + m_string[[{13}]] * current_power) % m_modulo.
+    ::// current_power := (current_power * m_multiplier) % m_modulo.
+    |-----------------------------.
+    ::// m_hash := (m_hash + m_string[[{14}]] * current_power) % m_modulo.
+    ::// current_power := (current_power * m_multiplier) % m_modulo.
+    ::// m_hash := (m_hash + m_string[[{15}]] * current_power) % m_modulo.
+    ::// current_power := (current_power * m_multiplier) % m_modulo.
+    |-----------------------------.
+    ::// m_hash := (m_hash + m_string[[{16}]] * current_power) % m_modulo.
+    ::// current_power := (current_power * m_multiplier) % m_modulo.
+    ::// m_hash := (m_hash + m_string[[{17}]] * current_power) % m_modulo.
+    ::// current_power := (current_power * m_multiplier) % m_modulo.
+    |-----------------------------.
+    ::// m_hash := (m_hash + m_string[[{18}]] * current_power) % m_modulo.
+    ::// current_power := (current_power * m_multiplier) % m_modulo.
+    ::// m_hash := (m_hash + m_string[[{19}]] * current_power) % m_modulo.
+    ::// current_power := (current_power * m_multiplier) % m_modulo.
+    |-----------------------------.
+    ::// m_hash := (m_hash + m_string[[{20}]] * current_power) % m_modulo.
+    ::// current_power := (current_power * m_multiplier) % m_modulo.
+    ::// m_hash := (m_hash + m_string[[{21}]] * current_power) % m_modulo.
+    ::// current_power := (current_power * m_multiplier) % m_modulo.
+    |-----------------------------.
+    ::// m_hash := (m_hash + m_string[[{22}]] * current_power) % m_modulo.
+    ::// current_power := (current_power * m_multiplier) % m_modulo.
+    ::// m_hash := (m_hash + m_string[[{23}]] * current_power) % m_modulo.
+    ::// current_power := (current_power * m_multiplier) % m_modulo.
+    |-----------------------------.
+    ::// m_hash := (m_hash + m_string[[{24}]] * current_power) % m_modulo.
+    ::// current_power := (current_power * m_multiplier) % m_modulo.
+    ::// m_hash := (m_hash + m_string[[{25}]] * current_power) % m_modulo.
+    ::// current_power := (current_power * m_multiplier) % m_modulo.
+    |-----------------------------.
+    ::// m_hash := (m_hash + m_string[[{26}]] * current_power) % m_modulo.
+    ::// current_power := (current_power * m_multiplier) % m_modulo.
+    ::// m_hash := (m_hash + m_string[[{27}]] * current_power) % m_modulo.
+    ::// current_power := (current_power * m_multiplier) % m_modulo.
+    |-----------------------------.
+    ::// m_hash := (m_hash + m_string[[{28}]] * current_power) % m_modulo.
+    ::// current_power := (current_power * m_multiplier) % m_modulo.
+    ::// m_hash := (m_hash + m_string[[{29}]] * current_power) % m_modulo.
+    ::// current_power := (current_power * m_multiplier) % m_modulo.
+    |-----------------------------.
+    ::// m_hash := (m_hash + m_string[[{30}]] * current_power) % m_modulo.
+    ::// current_power := (current_power * m_multiplier) % m_modulo.
+    ::// m_hash := (m_hash + m_string[[{31}]] * current_power) % m_modulo.
+    ::// current_power := (current_power * m_multiplier) % m_modulo.
+    |-----------------------------.
+    ::// m_hash := (m_hash + m_string[[{32}]] * current_power) % m_modulo.
+    ::// current_power := (current_power * m_multiplier) % m_modulo.
+    ::// m_hash := (m_hash + m_string[[{33}]] * current_power) % m_modulo.
+    ::// current_power := (current_power * m_multiplier) % m_modulo.
+    |-----------------------------.
+    ::// m_hash := (m_hash + m_string[[{34}]] * current_power) % m_modulo.
+    ::// current_power := (current_power * m_multiplier) % m_modulo.
+    ::// m_hash := (m_hash + m_string[[{35}]] * current_power) % m_modulo.
+    ::// current_power := (current_power * m_multiplier) % m_modulo.
+    |-----------------------------.
+    ::// m_hash := (m_hash + m_string[[{36}]] * current_power) % m_modulo.
+    ::// current_power := (current_power * m_multiplier) % m_modulo.
+    ::// m_hash := (m_hash + m_string[[{37}]] * current_power) % m_modulo.
+    ::// current_power := (current_power * m_multiplier) % m_modulo.
+    |-----------------------------.
+    ::// m_hash := (m_hash + m_string[[{38}]] * current_power) % m_modulo |.
+}
+return.
+Defined.
+Sync.
+
+Ursus Definition hash_40: UExpression PhantomType false.
+{
+    ::// var00 current_power: uint64 := {1} ;_|.
+    ::// m_hash := {0} ;_|.
+    |-----------------------------.
+    ::// m_hash := (m_hash + m_string[[{0}]] * current_power) % m_modulo.
+    ::// current_power := (current_power * m_multiplier) % m_modulo.
+    ::// m_hash := (m_hash + m_string[[{1}]] * current_power) % m_modulo.
+    ::// current_power := (current_power * m_multiplier) % m_modulo.
+    |-----------------------------.
+    ::// m_hash := (m_hash + m_string[[{2}]] * current_power) % m_modulo.
+    ::// current_power := (current_power * m_multiplier) % m_modulo.
+    ::// m_hash := (m_hash + m_string[[{3}]] * current_power) % m_modulo.
+    ::// current_power := (current_power * m_multiplier) % m_modulo.
+    |-----------------------------.
+    ::// m_hash := (m_hash + m_string[[{4}]] * current_power) % m_modulo.
+    ::// current_power := (current_power * m_multiplier) % m_modulo.
+    ::// m_hash := (m_hash + m_string[[{5}]] * current_power) % m_modulo.
+    ::// current_power := (current_power * m_multiplier) % m_modulo.
+    |-----------------------------.
+    ::// m_hash := (m_hash + m_string[[{6}]] * current_power) % m_modulo.
+    ::// current_power := (current_power * m_multiplier) % m_modulo.
+    ::// m_hash := (m_hash + m_string[[{7}]] * current_power) % m_modulo.
+    ::// current_power := (current_power * m_multiplier) % m_modulo.
+    |-----------------------------.
+    ::// m_hash := (m_hash + m_string[[{8}]] * current_power) % m_modulo.
+    ::// current_power := (current_power * m_multiplier) % m_modulo.
+    ::// m_hash := (m_hash + m_string[[{9}]] * current_power) % m_modulo.
+    ::// current_power := (current_power * m_multiplier) % m_modulo.
+    |-----------------------------.
+    ::// m_hash := (m_hash + m_string[[{10}]] * current_power) % m_modulo.
+    ::// current_power := (current_power * m_multiplier) % m_modulo.
+    ::// m_hash := (m_hash + m_string[[{11}]] * current_power) % m_modulo.
+    ::// current_power := (current_power * m_multiplier) % m_modulo.
+    |-----------------------------.
+    ::// m_hash := (m_hash + m_string[[{12}]] * current_power) % m_modulo.
+    ::// current_power := (current_power * m_multiplier) % m_modulo.
+    ::// m_hash := (m_hash + m_string[[{13}]] * current_power) % m_modulo.
+    ::// current_power := (current_power * m_multiplier) % m_modulo.
+    |-----------------------------.
+    ::// m_hash := (m_hash + m_string[[{14}]] * current_power) % m_modulo.
+    ::// current_power := (current_power * m_multiplier) % m_modulo.
+    ::// m_hash := (m_hash + m_string[[{15}]] * current_power) % m_modulo.
+    ::// current_power := (current_power * m_multiplier) % m_modulo.
+    |-----------------------------.
+    ::// m_hash := (m_hash + m_string[[{16}]] * current_power) % m_modulo.
+    ::// current_power := (current_power * m_multiplier) % m_modulo.
+    ::// m_hash := (m_hash + m_string[[{17}]] * current_power) % m_modulo.
+    ::// current_power := (current_power * m_multiplier) % m_modulo.
+    |-----------------------------.
+    ::// m_hash := (m_hash + m_string[[{18}]] * current_power) % m_modulo.
+    ::// current_power := (current_power * m_multiplier) % m_modulo.
+    ::// m_hash := (m_hash + m_string[[{19}]] * current_power) % m_modulo.
+    ::// current_power := (current_power * m_multiplier) % m_modulo.
+    |-----------------------------.
+    ::// m_hash := (m_hash + m_string[[{20}]] * current_power) % m_modulo.
+    ::// current_power := (current_power * m_multiplier) % m_modulo.
+    ::// m_hash := (m_hash + m_string[[{21}]] * current_power) % m_modulo.
+    ::// current_power := (current_power * m_multiplier) % m_modulo.
+    |-----------------------------.
+    ::// m_hash := (m_hash + m_string[[{22}]] * current_power) % m_modulo.
+    ::// current_power := (current_power * m_multiplier) % m_modulo.
+    ::// m_hash := (m_hash + m_string[[{23}]] * current_power) % m_modulo.
+    ::// current_power := (current_power * m_multiplier) % m_modulo.
+    |-----------------------------.
+    ::// m_hash := (m_hash + m_string[[{24}]] * current_power) % m_modulo.
+    ::// current_power := (current_power * m_multiplier) % m_modulo.
+    ::// m_hash := (m_hash + m_string[[{25}]] * current_power) % m_modulo.
+    ::// current_power := (current_power * m_multiplier) % m_modulo.
+    |-----------------------------.
+    ::// m_hash := (m_hash + m_string[[{26}]] * current_power) % m_modulo.
+    ::// current_power := (current_power * m_multiplier) % m_modulo.
+    ::// m_hash := (m_hash + m_string[[{27}]] * current_power) % m_modulo.
+    ::// current_power := (current_power * m_multiplier) % m_modulo.
+    |-----------------------------.
+    ::// m_hash := (m_hash + m_string[[{28}]] * current_power) % m_modulo.
+    ::// current_power := (current_power * m_multiplier) % m_modulo.
+    ::// m_hash := (m_hash + m_string[[{29}]] * current_power) % m_modulo.
+    ::// current_power := (current_power * m_multiplier) % m_modulo.
+    |-----------------------------.
+    ::// m_hash := (m_hash + m_string[[{30}]] * current_power) % m_modulo.
+    ::// current_power := (current_power * m_multiplier) % m_modulo.
+    ::// m_hash := (m_hash + m_string[[{31}]] * current_power) % m_modulo.
+    ::// current_power := (current_power * m_multiplier) % m_modulo.
+    |-----------------------------.
+    ::// m_hash := (m_hash + m_string[[{32}]] * current_power) % m_modulo.
+    ::// current_power := (current_power * m_multiplier) % m_modulo.
+    ::// m_hash := (m_hash + m_string[[{33}]] * current_power) % m_modulo.
+    ::// current_power := (current_power * m_multiplier) % m_modulo.
+    |-----------------------------.
+    ::// m_hash := (m_hash + m_string[[{34}]] * current_power) % m_modulo.
+    ::// current_power := (current_power * m_multiplier) % m_modulo.
+    ::// m_hash := (m_hash + m_string[[{35}]] * current_power) % m_modulo.
+    ::// current_power := (current_power * m_multiplier) % m_modulo.
+    |-----------------------------.
+    ::// m_hash := (m_hash + m_string[[{36}]] * current_power) % m_modulo.
+    ::// current_power := (current_power * m_multiplier) % m_modulo.
+    ::// m_hash := (m_hash + m_string[[{37}]] * current_power) % m_modulo.
+    ::// current_power := (current_power * m_multiplier) % m_modulo.
+    |-----------------------------.
+    ::// m_hash := (m_hash + m_string[[{38}]] * current_power) % m_modulo.
+    ::// current_power := (current_power * m_multiplier) % m_modulo.
+    ::// m_hash := (m_hash + m_string[[{39}]] * current_power) % m_modulo |.
+}
+return.
+Defined.
+Sync.
+
 (*
 uint64 result;
 function f(uint64 a, uint64 b) {
