run_experiments.sh
@@ -1,6 +1,7 @@
+JOBS=40
 dune cle
 ./clear_gen.sh
-(dune b --no-buffer; dune b --no-buffer; dune b --no-buffer; dune b --no-buffer; dune b --no-buffer; dune b --no-buffer) &> plots/output.txt
+(dune b --no-buffer -j $JOBS; dune b --no-buffer -j $JOBS; dune b --no-buffer -j $JOBS; dune b --no-buffer -j $JOBS; dune b --no-buffer -j $JOBS; dune b --no-buffer -j $JOBS) &> plots/output.txt
 cd plots
 ./plot.sh output.txt basic.txt 10
 ./plot.sh output.txt topdown.txt 10
@@ -8,4 +9,5 @@ cd plots
 ./plot.sh output.txt winners.txt 10
 ./plot.sh output.txt bottomup_naive.txt 10
 ./plot.sh output.txt bottomup_reductions.txt 10
+./plot.sh output.txt winners.txt
 cd ..
